LL1/Soundness.v
@@ -160,3 +160,4 @@ Proof.
   apply app_inv_tail in Happ.
   subst; auto.
 Qed.
+
